Reverted BoundVars.v relations to use a string specific version of In instead

src/Language/PlutusIR/Analysis/BoundVars.v
@@ -64,34 +64,18 @@ Instance appears_bound_in_ty_DecOpt_monotonicity x ty: DecOptSizeMonotonic (appe
 Proof. derive_mon. Qed.
 
 
-
-Inductive appears_bound_in_constrs (x : name) : list constructor -> Prop :=
-  | ABIC_Here  : forall t n cs,
-      appears_bound_in_constrs x ((Constructor (VarDecl x t) n) :: cs)
-  | ABIC_There : forall c' cs,
-      appears_bound_in_constrs x cs ->
-      appears_bound_in_constrs x (c' :: cs).
-
-QCDerive DecOpt for (appears_bound_in_constrs x ls).
-
-Instance appears_bound_in_constrs_DecOpt_sound x ty: DecOptSoundPos (appears_bound_in_constrs x ty).
-Proof. derive_sound. Qed.
-
-Instance appears_bound_in_constrs_DecOpt_complete x ty: DecOptCompletePos (appears_bound_in_constrs x ty).
-Proof. derive_complete. Qed.
-
-Instance appears_bound_in_constrs_DecOpt_monotonicity x ty: DecOptSizeMonotonic (appears_bound_in_constrs x ty).
-Proof. derive_mon. Qed.
-
-
-
-(* QuickChick will fail to derive a checker for appears_bound_in if this application
+(* Old comment: QuickChick will fail to derive a checker for appears_bound_in if this application
  * occurs directly in the constructor. This is because QuickChick will try and match
  * 'bv_constructor' with the variables bound by the 'forall', which will fail.
  *
  * In short, only the function is allowed to be defined outside the constructor, and
  * any variables applied to the function should be bound as quantified variables.
  *)
+Fixpoint bv_constructors (cs : list constructor) : list string :=
+  match cs with
+  | [] => []
+  | (Constructor (VarDecl x _) _) :: cs' => x :: bv_constructors cs'
+  end.
 
 Inductive appears_bound_in_tm (x : name) : Term -> Prop :=
   | ABITM_LamAbs1 : forall T t,
@@ -128,12 +112,9 @@ Inductive appears_bound_in_tm (x : name) : Term -> Prop :=
   | ABITM_Let_TermBind2 : forall recty stricty y T t bs t0,
       appears_bound_in_tm x t ->
       appears_bound_in_tm x (Let recty (TermBind stricty (VarDecl y T) t :: bs) t0)
-  | ABITM_Let_DatatypeBindHere : forall recty XK YKs cs t0 bs,
-      appears_bound_in_tm x (Let recty (DatatypeBind (Datatype XK YKs x cs) :: bs) t0)
-  | ABITM_Let_DatatypeBindThere : forall recty XK YKs mfunc cs t0 bs,
-      appears_bound_in_constrs x cs ->
-      appears_bound_in_tm x (Let recty (DatatypeBind (Datatype XK YKs mfunc cs) :: bs) t0).
-  
+  | ABITM_Let_DatatypeBind : forall recty XK YKs mfunc cs t0 bs,
+      NameIn x (mfunc :: bv_constructors cs) ->
+      appears_bound_in_tm x (Let recty (DatatypeBind (Datatype XK YKs mfunc cs) :: bs) t0).  
 
 (* Necessary since 'In' has strings as arguments *)
 (* TODO: move these elsewhere? In favour of deriving these once in a central place?*)
@@ -142,7 +123,6 @@ QCDerive EnumSized for string.
 
 QCDerive DecOpt for (appears_bound_in_tm x tm).
 
-(* TODO: finishes, but does not finalize a proof :( *)
 Instance appears_bound_in_tm_DecOpt_sound x tm: DecOptSoundPos (appears_bound_in_tm x tm).
 Proof. derive_sound. Qed.
 
@@ -199,7 +179,7 @@ Inductive appears_bound_in_ann (X : tyname) : Term -> Prop :=
       appears_bound_in_ann X (Let recty nil t0)
   | ABIA_Let_Cons : forall recty b bs t0,
       appears_bound_in_ann X (Let recty bs t0) ->
-        appears_bound_in_ann X (Let recty (b :: bs) t0)
+      appears_bound_in_ann X (Let recty (b :: bs) t0)
   | ABIA_Let_TermBind1 : forall recty stricty x T t bs t0,
       appears_bound_in_ty X T ->
       appears_bound_in_ann X (Let recty (TermBind stricty (VarDecl x T) t :: bs) t0)
@@ -212,18 +192,17 @@ Inductive appears_bound_in_ann (X : tyname) : Term -> Prop :=
       appears_bound_in_ty X T ->
       appears_bound_in_ann X (Let recty (TypeBind (TyVarDecl Y K) T :: bs) t0)
   | ABIA_Let_DatatypeBind : forall recty K YKs mfunc cs t0 bs,
-      appears_bound_in_ann X (Let recty (DatatypeBind (Datatype (TyVarDecl X K) YKs mfunc cs) :: bs) t0) 
-      .
+      appears_bound_in_ann X (Let recty (DatatypeBind (Datatype (TyVarDecl X K) YKs mfunc cs) :: bs) t0).
 
 QCDerive DecOpt for (appears_bound_in_ann x tm).
 
 Instance appears_bound_in_ann_DecOpt_sound x tm: DecOptSoundPos (appears_bound_in_ann x tm).
 Proof. derive_sound. Qed.
 
-Instance appears_bound_in_ann_DecOpt_complete x ty: DecOptCompletePos (appears_bound_in_ann x ty).
+Instance appears_bound_in_ann_DecOpt_complete x tm: DecOptCompletePos (appears_bound_in_ann x tm).
 Proof. derive_complete. Qed.
 
-Instance appears_bound_in_ann_DecOpt_monotonic x ty: DecOptSizeMonotonic (appears_bound_in_ann x ty).
+Instance appears_bound_in_ann_DecOpt_monotonic x tm: DecOptSizeMonotonic (appears_bound_in_ann x tm).
 Proof. derive_mon. Qed.
 
 
@@ -387,18 +366,22 @@ Proof with eauto using appears_bound_in_tm.
     destruct dtd.
     apply Forall_cons.
     + intros.
-      apply ABITM_Let_DatatypeBindHere.
+      apply ABITM_Let_DatatypeBind.
+      constructor...
     + apply Forall_forall.
       intros.
-      apply ABITM_Let_DatatypeBindThere.
-      induction l0; inversion H; induction a; induction v.
-      * subst.
-        apply ABIC_Here.
-      * destruct H.
-        -- subst. apply ABIC_Here.
-        -- apply ABIC_There.
-           apply IHl0.
-           auto.
+      apply ABITM_Let_DatatypeBind.
+      apply NameIn_In_string_equal.
+      apply in_cons.
+      induction l0; try assumption.
+      destruct a.
+      destruct v.
+      induction H; subst; simpl.
+     * left. 
+       reflexivity.
+     * right. 
+       apply IHl0.
+       apply H.
 Qed.
 
 Inductive decide {a : Type} (P : a -> Type) (x : a) :=
